graph monad (to be improved)

FormattedGraph/Graph.lean
@@ -7,10 +7,10 @@ variable {ν : Type*} {ε : Type*} [DecidableEq ν] [DecidableEq ε]
 
 /--
 finite directed graph
-* `ν`: the type of all possible vertices
+* `ν`: the type of all possible nodes
 * `ε`: the type of all possible edges
 * `ep`: the endpoints of each edge in `ε`
-* `V`: the finite set of vertices
+* `V`: the finite set of nodes
 * `E`: the finite set of edges
 * `h`: the hypothesis that the endpoints of each edge in `E` is in `V`
 -/
@@ -28,9 +28,9 @@ def discrete (ep : ε → ν × ν) (V : Finset ν) : Graph ep where
   h := by intro _ he; simp at he
 
 /--
-`empty ep`: the empty graph, i.e., the one with no vertices and edges.
+`empty ep`: the empty graph, i.e., the one with no nodes and edges.
 -/
-def empty (ep : ε → ν × ν) : Graph ep :=
+def empty {ep : ε → ν × ν} : Graph ep :=
   discrete ep ∅
 
 /--
@@ -118,6 +118,25 @@ def push_forward_edge {ep : ε → ν × ν}
     (G : Graph ep) : Graph ep :=
   push_forward f.toPushForwardStruct G
 
+/--
+`add_edge_safe_raw e G h1 h2`: to add an edge `e` to a graph `G`
+  under the assumptions that both endpoints of `e` are in `G`.
+
+This operation preserves the node set.
+-/
+def add_edge_safe {ep : ε → ν × ν} (e : ε)
+    (G : Graph ep)
+    (h1 : (ep e).1 ∈ G.V)
+    (h2 : (ep e).2 ∈ G.V)
+  : Graph ep where
+  V := G.V
+  E := G.E ∪ {e}
+  h := by
+    intro _ h; simp at h
+    rcases h with h | h
+    . subst h; constructor <;> assumption
+    . exact G.h h
+
 end FiniteDirectedGraph
 
 
@@ -128,7 +147,7 @@ end FiniteDirectedGraph
 
 
 
-namespace WithData
+namespace GraphWithData
 
 variable {ν : Type*} {ε : Type*} [DecidableEq ν] [DecidableEq ε]
 
@@ -143,18 +162,28 @@ variable [node_data_type : NodeData ν] [edge_data_type : EdgeData ε]
 
 abbrev δ (α : Type*) [data_type : Data α] := data_type.data_type
 
-structure GraphWithData (ep : ε → ν × ν)
+end GraphWithData
+
+structure GraphWithData
+  {ν : Type*} {ε : Type*}
+  [DecidableEq ν] [DecidableEq ε]
+  [node_data_type : GraphWithData.NodeData ν]
+  [edge_data_type : GraphWithData.EdgeData ε]
+  (ep : ε → ν × ν)
     extends FiniteDirectedGraph.Graph ep where
-  data_v : V → δ ν
-  data_e : E → δ ε
+  data_v : V → GraphWithData.δ ν
+  data_e : E → GraphWithData.δ ε
 
 namespace GraphWithData
 
+variable {ν : Type*} {ε : Type*} [DecidableEq ν] [DecidableEq ε]
+variable [node_data_type : NodeData ν] [edge_data_type : EdgeData ε]
+
 /--
-`empty ep`: the empty graph, i.e., the one with no vertices and edges.
+`empty ep`: the empty graph, i.e., the one with no nodes and edges.
 -/
-def empty (ep : ε → ν × ν) : GraphWithData ep where
-  toGraph := FiniteDirectedGraph.empty ep
+def empty {ep : ε → ν × ν} : GraphWithData ep where
+  toGraph := FiniteDirectedGraph.empty
   data_v := fun ⟨_, h⟩ => (Finset.notMem_empty _ h).elim
   data_e := fun ⟨_, h⟩ => (Finset.notMem_empty _ h).elim
 
@@ -184,7 +213,8 @@ def add_node {ep : ε → ν × ν} (v : ν) (dv : δ ν)
 /--
 `add_edge e de dv G`: to add an edge `e` with data `de` to a graph `G`.
 If `e` is already in `G`, then nothing happens.
-If some of the endpoints of `e` is not in `G`, then add it with data `dv`.
+If some of the endpoints of `e` is not in `G`, then add it with data `dv`,
+  which serves as a default value.
 -/
 def add_edge {ep : ε → ν × ν} (e : ε) (de : δ ε) (dv : δ ν)
     (G : GraphWithData ep) : GraphWithData ep where
@@ -258,6 +288,204 @@ def edit_edge {ep : ε → ν × ν} (e : ε) (de : δ ε)
     if e' = e then de
     else G.data_e ⟨e', h⟩
 
+inductive GraphWithDataError (ν ε : Type*) where
+  | add_node_existing (v : ν)
+  | add_edge_existing (e : ε)
+  | add_edge_start_point_missing (e : ε)
+  | add_edge_end_point_missing (e : ε)
+  | remove_node_missing (v : ν)
+  | remove_edge_missing (e : ε)
+  | edit_node_missing (v : ν)
+  | edit_edge_missing (e : ε)
+
+def GraphWithDataM (ep : ε → ν × ν) :=
+  Except (GraphWithDataError ν ε) (GraphWithData ep)
+
+/--
+`add_node v dv G`: to add a node `v` with data `dv` to a graph `G`.
+If `v` is already in `G`, then error `add_node_existing v` will be thrown out.
+-/
+def add_node_safe {ep : ε → ν × ν} (v : ν) (dv : δ ν)
+    (G : GraphWithData ep) : GraphWithDataM ep :=
+  if v ∈ G.V
+  then .error $ .add_node_existing v
+  else .ok (G.add_node v dv)
+
+/--
+`add_edge_safe e de G`: to add an edge `e` with data `de` to a graph `G`.
+If `e` is already in `G`, then error `add_node_existing e` will be thrown out.
+If some of the endpoints of `e` is not in `G`, then error
+  `add_edge_start_point_missing` or `add_edge_end_point_missing` will be thrown
+  out.
+-/
+def add_edge_safe {ep : ε → ν × ν} (e : ε) (de : δ ε)
+    (G : GraphWithData ep) : GraphWithDataM ep :=
+  if e ∈ G.E then .error $ .add_edge_existing e
+  else if h1 : (ep e).1 ∈ G.V then
+    if h2 : (ep e).2 ∈ G.V then
+      .ok ⟨
+        FiniteDirectedGraph.add_edge_safe e G.toGraph h1 h2,
+        G.data_v,
+        fun ⟨e', _⟩ =>
+          if he' : e' ∈ G.E
+          then G.data_e ⟨e', he'⟩
+          else de
+      ⟩
+    else .error $ .add_edge_end_point_missing e
+  else .error $ .add_edge_start_point_missing e
+
 end GraphWithData
 
-end WithData
+
+
+
+
+
+namespace test
+
+open GraphWithData
+
+namespace Shape
+
+structure Coordinate where
+  x : Float
+  y : Float
+
+structure Size where
+  size : Float
+  h : size > 0 := by native_decide
+
+end Shape
+
+structure NodeFormat where
+  size : Shape.Size
+  pos : Shape.Coordinate
+
+structure NodeDataType where
+  content : String
+  format : NodeFormat
+
+structure EdgeFormat where
+  pos1 : Shape.Coordinate
+  pos2 : Shape.Coordinate
+
+structure EdgeDataType where
+  content : String
+  format : EdgeFormat
+
+instance : NodeData Nat where
+  data_type := NodeDataType
+
+instance : EdgeData (Nat × Nat) where
+  data_type := EdgeDataType
+
+def ep : Nat × Nat → Nat × Nat := id
+
+def NodeDataDefault : NodeDataType where
+  content := ""
+  format := ⟨.mk 1, ⟨0, 0⟩⟩
+
+def NodeDataLxy : NodeDataType where
+  content := "Liu Xiaoyang"
+  format := ⟨.mk 10, ⟨1, 0⟩⟩
+
+def NodeDataDzn : NodeDataType where
+  content := "Dong Zineng"
+  format := ⟨.mk 10, ⟨-1, 0⟩⟩
+
+def EdgeData.mk' (content : String) (dv1 dv2 : NodeDataType) : EdgeDataType where
+  content := content
+  format := ⟨dv1.format.pos, dv2.format.pos⟩
+
+def graphExample : GraphWithData ep :=
+  (((empty
+  ).add_node
+    1 NodeDataLxy
+  ).add_node
+    2 NodeDataDzn
+  ).add_edge
+    (1,2)
+    (EdgeData.mk' "" NodeDataLxy NodeDataDzn)
+    NodeDataDefault
+/--
+`add_edge_safe e de G`: to add an edge `e` with data `de` to a graph `G`.
+If `e` is already in `G`, then error `add_node_existing e` will be thrown out.
+If some of the endpoints of `e` is not in `G`, then error
+  `add_edge_start_point_missing` or `add_edge_end_point_missing` will be thrown
+  out.
+-/
+def add_edge_safe' (e : Nat × Nat) (contents : String)
+    (G : GraphWithData ep) : GraphWithDataM ep :=
+  if e ∈ G.E then .error $ .add_edge_existing e
+  else if h1 : (ep e).1 ∈ G.V then
+    if h2 : (ep e).2 ∈ G.V then
+      .ok ⟨
+        FiniteDirectedGraph.add_edge_safe e G.toGraph h1 h2,
+        G.data_v,
+        fun ⟨e', _⟩ =>
+          if he' : e' ∈ G.E
+          then G.data_e ⟨e', he'⟩
+          else ⟨contents, ⟨
+              (G.data_v ⟨(ep e).1, h1⟩).format.pos,
+              (G.data_v ⟨(ep e).2, h2⟩).format.pos
+            ⟩⟩
+      ⟩
+    else .error $ .add_edge_end_point_missing e
+  else .error $ .add_edge_start_point_missing e
+
+def graphExampleM : GraphWithDataM ep := do
+  let G0 ← (pure empty)
+  let G1 ← G0.add_node_safe 1 NodeDataLxy
+  let G2 ← G1.add_node_safe 2 NodeDataDzn
+  let G3 ← add_edge_safe' (1,2) "" G2
+  pure G3
+
+theorem except_ok_fold (x : α) (m : α → @Except β α)
+  : (do
+      let y ← Except.ok x
+      m y)
+    = m x :=
+  rfl
+
+example : graphExampleM = .ok graphExample := by
+  have h1 : 1 ∉ (empty (ep := ep)).V := by
+    apply Finset.notMem_empty
+  have h2 : 2 ∉ (add_node 1 NodeDataLxy (empty (ep := ep))).V := by
+    unfold add_node; simp
+    unfold FiniteDirectedGraph.add_node; simp
+    apply Finset.notMem_empty
+  have h3 :
+    (1, 2) ∉
+    (add_node 2 NodeDataDzn (add_node 1 NodeDataLxy (empty (ep := ep)))).E
+  := by
+    unfold add_node; simp
+    unfold FiniteDirectedGraph.add_node; simp
+    apply Finset.notMem_empty
+  have h4 :
+    (ep (1, 2)).1 ∈
+    (add_node 2 NodeDataDzn (add_node 1 NodeDataLxy (empty (ep := ep)))).V
+  := by
+    unfold add_node; simp
+    unfold FiniteDirectedGraph.add_node; simp
+    left; rfl
+  have h5 :
+    (ep (1, 2)).2 ∈
+    (add_node 2 NodeDataDzn (add_node 1 NodeDataLxy (empty (ep := ep)))).V
+  := by
+    unfold add_node; simp
+    unfold FiniteDirectedGraph.add_node; simp
+    right; left; rfl
+  unfold graphExampleM
+  unfold graphExample
+  unfold add_node_safe at *
+  unfold add_edge_safe' at *
+  unfold add_node at *
+  unfold add_edge at *
+  simp [h1]; rw [except_ok_fold]
+  simp [h2]; rw [except_ok_fold]
+  simp [h3]
+  simp [h4]
+  simp [h5]
+  rfl
+
+end test
